feat: add MLIR syntax for PaperExamples IR

SSA/Projects/PaperExamples/PaperExamples.lean
@@ -1,6 +1,11 @@
+import Qq
+import Lean
 import Mathlib.Logic.Function.Iterate
 import SSA.Core.Framework
 import SSA.Core.Util
+import SSA.Projects.InstCombine.LLVM.Transform
+import SSA.Projects.MLIRSyntax.AST
+import SSA.Projects.MLIRSyntax.EDSL
 
 set_option pp.proofs false
 set_option pp.proofs.withType false
@@ -51,6 +56,79 @@ def add {Γ : Ctxt _} (e₁ e₂ : Var Γ .int) : Expr Op Γ .int :=
 
 attribute [local simp] Ctxt.snoc
 
+namespace MLIR2Simple
+
+def mkTy : MLIR.AST.MLIRType φ → MLIR.AST.ExceptM Op Ty
+  | MLIR.AST.MLIRType.int MLIR.AST.Signedness.Signless w => do
+    return .int
+  | _ => throw .unsupportedType
+
+instance instTransformTy : MLIR.AST.TransformTy Op Ty 0 where
+  mkTy := mkTy
+
+def mkExpr (Γ : Ctxt Ty) (opStx : MLIR.AST.Op 0) : MLIR.AST.ReaderM Op (Σ ty, Expr Op Γ ty) := do
+  match opStx.name with
+  | "const" =>
+    match opStx.attrs.find_int "value" with
+    | .some (v, _ty) => return ⟨.int, cst v⟩
+    | .none => throw <| .generic s!"expected 'const' to have int attr 'value', found: {repr opStx}"
+  | "add" =>
+    match opStx.args with
+    | v₁Stx::v₂Stx::[] =>
+      let ⟨.int, v₁⟩ ← MLIR.AST.TypedSSAVal.mkVal Γ v₁Stx
+      let ⟨.int, v₂⟩ ← MLIR.AST.TypedSSAVal.mkVal Γ v₂Stx
+      return ⟨.int, add v₁ v₂⟩
+    | _ => throw <| .generic s!"expected two operands for `add`, found #'{opStx.args.length}' in '{repr opStx.args}'"
+  | _ => throw <| .unsupportedOp s!"unsupported operation {repr opStx}"
+
+instance : MLIR.AST.TransformExpr Op Ty 0 where
+  mkExpr := mkExpr
+
+def mkReturn (Γ : Ctxt Ty) (opStx : MLIR.AST.Op 0) : MLIR.AST.ReaderM Op (Σ ty, Com Op Γ ty) :=
+  if opStx.name == "return"
+  then match opStx.args with
+  | vStx::[] => do
+    let ⟨ty, v⟩ ← MLIR.AST.TypedSSAVal.mkVal Γ vStx
+    return ⟨ty, Com.ret v⟩
+  | _ => throw <| .generic s!"Ill-formed return statement (wrong arity, expected 1, got {opStx.args.length})"
+  else throw <| .generic s!"Tried to build return out of non-return statement {opStx.name}"
+
+instance : MLIR.AST.TransformReturn Op Ty 0 where
+  mkReturn := mkReturn
+
+open InstCombine (Op Ty) in
+
+def mlir2simple (reg : MLIR.AST.Region 0) :
+    MLIR.AST.ExceptM Op (Σ (Γ : Ctxt Ty) (ty : Ty), Com Op Γ ty) := MLIR.AST.mkCom reg
+
+open Qq MLIR AST Lean Elab Term Meta in
+elab "[toy_icom| " reg:mlir_region "]" : term => do
+  let ast_stx ← `([mlir_region| $reg])
+  let ast ← elabTermEnsuringTypeQ ast_stx q(Region 0)
+  let mvalues ← `(⟨[], by rfl⟩)
+  -- let mvalues : Q(Vector Nat 0) ← elabTermEnsuringType mvalues q(Vector Nat 0)
+  let com := q(ToyNoRegion.MLIR2Simple.mlir2simple $ast)
+  synthesizeSyntheticMVarsNoPostponing
+  let com : Q(MLIR.AST.ExceptM Op (Σ (Γ' : Ctxt Ty) (ty : Ty), Com Op Γ' ty)) ←
+    withTheReader Core.Context (fun ctx => { ctx with options := ctx.options.setBool `smartUnfolding false }) do
+      withTransparency (mode := TransparencyMode.all) <|
+        return ←reduce com
+  let comExpr : Expr := com
+  trace[Meta] com
+  trace[Meta] comExpr
+  match comExpr.app3? ``Except.ok with
+  | .some (_εexpr, _αexpr, aexpr) =>
+      match aexpr.app4? ``Sigma.mk with
+      | .some (_αexpr, _βexpr, _fstexpr, sndexpr) =>
+        match sndexpr.app4? ``Sigma.mk with
+        | .some (_αexpr, _βexpr, _fstexpr, sndexpr) =>
+            return sndexpr
+        | .none => throwError "Found `Except.ok (Sigma.mk _ WRONG)`, Expected (Except.ok (Sigma.mk _ (Sigma.mk _ _))"
+      | .none => throwError "Found `Except.ok WRONG`, Expected (Except.ok (Sigma.mk _ _))"
+  | .none => throwError "Expected `Except.ok`, found {comExpr}"
+
+end MLIR2Simple
+
 /-- x + 0 -/
 def lhs : Com Op (Ctxt.ofList [.int]) .int :=
    -- %c0 = 0
@@ -59,6 +137,20 @@ def lhs : Com Op (Ctxt.ofList [.int]) .int :=
   Com.lete (add ⟨1, by simp [Ctxt.snoc]⟩ ⟨0, by simp [Ctxt.snoc]⟩ ) <|
   -- return %out
   Com.ret ⟨0, by simp [Ctxt.snoc]⟩
+
+open MLIR AST MLIR2Simple in
+/-- Same code, written in MLIR syntax. -/
+def lhs_stx : Com Op (Ctxt.ofList [.int]) .int :=
+  [toy_icom| {
+    ^bb0(%x : i32):
+      %c0 = "const" () { value = 0 : i32 } : () -> i32
+      %out = "add" (%x, %c0) : (i32, i32) -> i32
+      "return" (%out) : (i32) -> (i32)
+  }]
+
+/-- Our MLIR syntax elaboration produces what we expect. -/
+theorem hlhs_stx : lhs = lhs_stx := rfl
+
 
 /-- x -/
 def rhs : Com Op (Ctxt.ofList [.int]) .int :=
